TseitinProofs.fst
@@ -12,29 +12,6 @@ open TseitinCore
 
 
 
-// let rec append_valid_cnf_formulas (f1 : list (list int)) (f2 : list (list int))
-//     : Lemma (requires valid_cnf_formula f1 /\ valid_cnf_formula f2)
-//             (ensures valid_cnf_formula (f1 @ f2))
-//     = if L.length f1 = 0 then ()
-//       else append_valid_cnf_formulas (tl f1) f2
-
-
-// let rec append_variables_in_interval (f1 : list (list int)) (f2 : list (list int))
-//                                      (n:nat) (start_interval:nat) (end_interval:nat)
-//     : Lemma (requires n <= start_interval /\ start_interval <= end_interval /\
-//                       valid_cnf_formula f1 /\ valid_cnf_formula f2 /\
-//                       variables_in_interval f1 n start_interval end_interval /\
-//                       variables_in_interval f2 n start_interval end_interval)
-//             (ensures valid_cnf_formula (f1 @ f2) /\ variables_in_interval (f1 @ f2) n start_interval end_interval)
-//     = append_valid_cnf_formulas f1 f2;
-//       if f1 = [] then ()
-//       else 
-//       (
-//           append_valid_cnf_formulas (L.tl f1) f2;
-//           append_variables_in_interval (tl f1) f2 n start_interval end_interval
-//       )
-
-
 let not_clauses_in_interval (v1:int) (v:int) (n:nat) (start_interval:nat) (end_interval:nat)
     : Lemma (requires n <= start_interval /\ start_interval <= v &&
                       valid_variable v1 && valid_variable v &&
@@ -44,29 +21,9 @@ let not_clauses_in_interval (v1:int) (v:int) (n:nat) (start_interval:nat) (end_i
     = ()
 
 
-// let aux (tau : list bool) 
-//         (f1:formula_t) (rf1 : list (list int)) (v1:int) (n:nat)
-//         (start_interval:nat) (end_interval:nat) (rf : list (list int)) (v:int)
-//     : Lemma (requires n <= start_interval /\ start_interval <= v /\
-//                       valid f1 rf1 v1 n start_interval v /\
-//                       tseitin_same_value f1 rf1 v1 n start_interval v /\
-//                       rf = rf1 @ (not_clauses v1 v) /\
-//                       end_interval = v + 1 /\
-//                       valid_cnf_formula rf /\
-//                       L.length tau >= end_interval /\
-//                       variables_up_to_cnf_formula rf (L.length tau) /\
-//                       truth_value_cnf_formula rf tau)
-//             (ensures variables_up_to (Not f1) (L.length tau) &&
-//                      variables_up_to_literal (pos_var_to_lit v) (L.length tau) &&
-//                      truth_value_literal (pos_var_to_lit v) tau = truth_value (Not f1) tau)
-//     = variables_up_to_monotone f1 n (L.length tau);
-//       assert (truth_value_literal (pos_var_to_lit v1) tau = truth_value f1 tau);
-//       lemma_not_clauses v1 v tau;
-//       assert (truth_value_literal (pos_var_to_lit v) tau = truth_value (Not f1) tau)
-
-
 let prove_same_value_not (f1:formula_t) (rf1 : list (list int)) (v1:int) (n:nat)
-                         (start_interval:nat) (end_interval:nat) (rf : list (list int)) (v:int)
+                         (start_interval:nat) (v:int) (end_interval:nat)
+                         (rf : list (list int)) 
     : Lemma (requires n <= start_interval /\ start_interval <= v /\
                       valid f1 rf1 v1 n start_interval v /\
                       tseitin_same_value f1 rf1 v1 n start_interval v /\
@@ -75,18 +32,21 @@ let prove_same_value_not (f1:formula_t) (rf1 : list (list int)) (v1:int) (n:nat)
             (ensures valid (Not f1) rf v n start_interval end_interval /\
                      tseitin_same_value (Not f1) rf v n start_interval end_interval)
     = append_valid_cnf_formulas rf1 (not_clauses v1 v);
-      variables_in_interval_monotone rf1 n start_interval v end_interval;
+      variables_in_interval_monotone rf1 n start_interval start_interval v end_interval;
       not_clauses_in_interval v1 v n start_interval end_interval;
       append_variables_in_interval rf1 (not_clauses v1 v) n start_interval end_interval;
       assert (valid (Not f1) rf v n start_interval end_interval);
 
       let aux (tau : list bool) 
-          : Lemma (requires L.length tau >= end_interval /\
+          : Lemma (requires L.length tau >= end_interval &&
                             truth_value_cnf_formula rf tau)
                   (ensures variables_up_to (Not f1) (L.length tau) &&
                            variables_up_to_literal (pos_var_to_lit v) (L.length tau) &&
                            truth_value_literal (pos_var_to_lit v) tau = truth_value (Not f1) tau)
           = variables_up_to_monotone f1 n (L.length tau);
+            // assert (variables_in_interval rf n start_interval end_interval);
+            // variables_in_interval_monotone rf n start_interval start_interval v end_interval;
+            assert (tseitin_same_value f1 rf v1 n start_interval end_interval);
             assert (truth_value_literal (pos_var_to_lit v1) tau = truth_value f1 tau);
             lemma_not_clauses v1 v tau;
             assert (truth_value_literal (pos_var_to_lit v) tau = truth_value (Not f1) tau)
@@ -94,251 +54,515 @@ let prove_same_value_not (f1:formula_t) (rf1 : list (list int)) (v1:int) (n:nat)
       forall_intro (move_requires aux)
 
 
-
-// let prove_same_value_or (f1:formula_t) (rf1 : list (list int)) (v1:int)
-//                         (f2:formula_t) (rf2 : list (list int)) (v2:int)
-//                         (n:nat) (start_interval:nat) (mid:nat) (end_interval:nat)
-//                         (v:int) (rf : list (list int))
-//     : Lemma (requires n <= start_interval /\ start_interval <= mid /\ mid <= v /\
-//                       valid f1 rf1 v1 n start_interval mid /\
-//                       tseitin_same_value f1 rf1 v1 n start_interval mid /\
-//                       valid f2 rf2 v2 n mid v /\
-//                       tseitin_same_value f2 rf2 v2 n mid v /\
-//                       rf = rf1 @ rf2 @ (or_clauses v1 v2 v) /\
-//                       end_interval = v + 1)
-//             (ensures valid (Or f1 f2) rf v n start_interval end_interval /\
-//                      tseitin_same_value (Or f1 f2) rf v n start_interval end_interval)
-//     = LP.append_assoc rf1 rf2 (or_clauses v1 v2 v);
-//       append_valid_cnf_formulas rf1 rf2;
-//       append_valid_cnf_formulas (rf1 @ rf2) (or_clauses v1 v2 v);
-//       // assert (variables_in_interval rf n start_interval end_interval);
-//       // assert (valid (Or f1 f2) rf v n start_interval end_interval);
-
-//       let aux (tau : list bool) 
-//           : Lemma (requires L.length tau >= end_interval /\
-//                             truth_value_cnf_formula rf tau)
-//                   (ensures truth_value_literal (pos_var_to_lit v) tau = truth_value (Or f1 f2) tau)
-//           = assert (variables_up_to_cnf_formula rf (L.length tau));
-//             variables_up_to_monotone f1 n (L.length tau);
-//             variables_up_to_monotone f2 n (L.length tau);
-//             assert (truth_value_literal (pos_var_to_lit v1) tau = truth_value f1 tau);
-//             assert (truth_value_literal (pos_var_to_lit v2) tau = truth_value f2 tau);
-//             lemma_or_clauses v1 v2 v tau;
-//             assert (truth_value_literal (pos_var_to_lit v) tau = truth_value (Or f1 f2) tau)
-//       in
-//       forall_intro (move_requires aux)
+let or_clauses_in_interval (v1:int) (v2:int) (v:int) (n:nat) (start_interval:nat) (mid:nat) (end_interval:nat)
+    : Lemma (requires n <= start_interval && start_interval <= mid && mid <= v &&
+                      valid_variable v1 && valid_variable v2 && valid_variable v &&
+                      variable_in_interval v1 n start_interval mid &&
+                      variable_in_interval v2 n mid v &&
+                      end_interval = v + 1)
+            (ensures variables_in_interval (or_clauses v1 v2 v) n start_interval end_interval)
+    = ()
 
 
-// let prove_same_value_and (f1:formula_t) (rf1 : list (list int)) (v1:int)
-//                          (f2:formula_t) (rf2 : list (list int)) (v2:int)
-//                          (n:nat) (start_interval:nat) (mid:nat) (end_interval:nat)
-//                          (v:int) (rf : list (list int))
-//     : Lemma (requires n <= start_interval /\ start_interval <= mid /\ mid <= v /\
-//                       valid f1 rf1 v1 n start_interval mid /\
-//                       tseitin_same_value f1 rf1 v1 n start_interval mid /\
-//                       valid f2 rf2 v2 n mid v /\
-//                       tseitin_same_value f2 rf2 v2 n mid v /\
-//                       rf = rf1 @ rf2 @ (and_clauses v1 v2 v) /\
-//                       end_interval = v + 1)
-//             (ensures valid (And f1 f2) rf v n start_interval end_interval /\
-//                      tseitin_same_value (And f1 f2) rf v n start_interval end_interval)
-//     = LP.append_assoc rf1 rf2 (and_clauses v1 v2 v);
-//       append_valid_cnf_formulas rf1 rf2;
-//       append_valid_cnf_formulas (rf1 @ rf2) (and_clauses v1 v2 v);
-//       // assert (variables_in_interval rf n start_interval end_interval);
-//       // assert (valid (And f1 f2) rf v n start_interval end_interval);
+let prove_same_value_or (f1:formula_t) (rf1 : list (list int)) (v1:int)
+                        (f2:formula_t) (rf2 : list (list int)) (v2:int)
+                        (n:nat) (start_interval:nat) (mid:nat) (end_interval:nat)
+                        (v:int) (rf : list (list int))
+    : Lemma (requires n <= start_interval /\ start_interval <= mid /\ mid <= v /\
+                      valid f1 rf1 v1 n start_interval mid /\
+                      tseitin_same_value f1 rf1 v1 n start_interval mid /\
+                      valid f2 rf2 v2 n mid v /\
+                      tseitin_same_value f2 rf2 v2 n mid v /\
+                      rf = rf1 @ rf2 @ (or_clauses v1 v2 v) /\
+                      end_interval = v + 1)
+            (ensures valid (Or f1 f2) rf v n start_interval end_interval /\
+                     tseitin_same_value (Or f1 f2) rf v n start_interval end_interval)
+    = LP.append_assoc rf1 rf2 (or_clauses v1 v2 v);
+      append_valid_cnf_formulas rf1 rf2;
+      append_valid_cnf_formulas (rf1 @ rf2) (or_clauses v1 v2 v);
 
-//       let aux (tau : list bool) 
-//           : Lemma (requires L.length tau >= end_interval /\
-//                             truth_value_cnf_formula rf tau)
-//                   (ensures truth_value_literal (pos_var_to_lit v) tau = truth_value (And f1 f2) tau)
-//           = assert (variables_up_to_cnf_formula rf (L.length tau));
-//             variables_up_to_monotone f1 n (L.length tau);
-//             variables_up_to_monotone f2 n (L.length tau);
-//             assert (truth_value_literal (pos_var_to_lit v1) tau = truth_value f1 tau);
-//             assert (truth_value_literal (pos_var_to_lit v2) tau = truth_value f2 tau);
-//             lemma_and_clauses v1 v2 v tau;
-//             assert (truth_value_literal (pos_var_to_lit v) tau = truth_value (And f1 f2) tau)
-//       in
-//       forall_intro (move_requires aux)
+      variables_in_interval_monotone rf1 n start_interval start_interval mid end_interval;
+      variables_in_interval_monotone rf2 n mid start_interval v end_interval;
 
+      or_clauses_in_interval v1 v2 v n start_interval mid end_interval;
+      append_variables_in_interval rf1 rf2 n start_interval end_interval;
+      append_variables_in_interval (rf1 @ rf2) (or_clauses v1 v2 v) n start_interval end_interval;
 
-// let prove_same_value_implies (f1:formula_t) (rf1 : list (list int)) (v1:int)
-//                              (f2:formula_t) (rf2 : list (list int)) (v2:int)
-//                              (n:nat) (start_interval:nat) (mid:nat) (end_interval:nat)
-//                              (v:int) (rf : list (list int))
-//     : Lemma (requires n <= start_interval /\ start_interval <= mid /\ mid <= v /\
-//                       valid f1 rf1 v1 n start_interval mid /\
-//                       tseitin_same_value f1 rf1 v1 n start_interval mid /\
-//                       valid f2 rf2 v2 n mid v /\
-//                       tseitin_same_value f2 rf2 v2 n mid v /\
-//                       rf = rf1 @ rf2 @ (implies_clauses v1 v2 v) /\
-//                       end_interval = v + 1)
-//             (ensures valid (Implies f1 f2) rf v n start_interval end_interval /\
-//                      tseitin_same_value (Implies f1 f2) rf v n start_interval end_interval)
-//     = LP.append_assoc rf1 rf2 (implies_clauses v1 v2 v);
-//       append_valid_cnf_formulas rf1 rf2;
-//       append_valid_cnf_formulas (rf1 @ rf2) (implies_clauses v1 v2 v);
-//       // assert (variables_in_interval rf n start_interval end_interval);
-//       // assert (valid (Implies f1 f2) rf v n start_interval end_interval);
+      assert (valid (Or f1 f2) rf v n start_interval end_interval);
 
-//       let aux (tau : list bool) 
-//           : Lemma (requires L.length tau >= end_interval /\
-//                             truth_value_cnf_formula rf tau)
-//                   (ensures truth_value_literal (pos_var_to_lit v) tau = truth_value (Implies f1 f2) tau)
-//           = assert (variables_up_to_cnf_formula rf (L.length tau));
-//             variables_up_to_monotone f1 n (L.length tau);
-//             variables_up_to_monotone f2 n (L.length tau);
-//             assert (truth_value_literal (pos_var_to_lit v1) tau = truth_value f1 tau);
-//             assert (truth_value_literal (pos_var_to_lit v2) tau = truth_value f2 tau);
-//             lemma_and_clauses v1 v2 v tau;
-//             assert (truth_value_literal (pos_var_to_lit v) tau = truth_value (Implies f1 f2) tau)
-//       in
-//       forall_intro (move_requires aux)
+      let aux (tau : list bool) 
+          : Lemma (requires L.length tau >= end_interval &&
+                            truth_value_cnf_formula rf tau)
+                  (ensures variables_up_to (Or f1 f2) (L.length tau) &&
+                           variables_up_to_literal (pos_var_to_lit v) (L.length tau) &&truth_value_literal (pos_var_to_lit v) tau = truth_value (Or f1 f2) tau)
+          = assert (variables_up_to_cnf_formula rf (L.length tau));
+            variables_up_to_monotone f1 n (L.length tau);
+            variables_up_to_monotone f2 n (L.length tau);
+            assert (truth_value_literal (pos_var_to_lit v1) tau = truth_value f1 tau);
+            assert (truth_value_literal (pos_var_to_lit v2) tau = truth_value f2 tau);
+            lemma_or_clauses v1 v2 v tau;
+            assert (truth_value_literal (pos_var_to_lit v) tau = truth_value (Or f1 f2) tau)
+      in
+      forall_intro (move_requires aux)
 
 
-// let prove_same_value_dimplies (f1:formula_t) (rf1 : list (list int)) (v1:int)
-//                               (f2:formula_t) (rf2 : list (list int)) (v2:int)
-//                               (n:nat) (start_interval:nat) (mid:nat) (end_interval:nat)
-//                               (v:int) (rf : list (list int))
-//     : Lemma (requires n <= start_interval /\ start_interval <= mid /\ mid <= v /\
-//                       valid f1 rf1 v1 n start_interval mid /\
-//                       tseitin_same_value f1 rf1 v1 n start_interval mid /\
-//                       valid f2 rf2 v2 n mid v /\
-//                       tseitin_same_value f2 rf2 v2 n mid v /\
-//                       rf = rf1 @ rf2 @ (dimplies_clauses v1 v2 v) /\
-//                       end_interval = v + 1)
-//             (ensures valid (DImplies f1 f2) rf v n start_interval end_interval /\
-//                      tseitin_same_value (DImplies f1 f2) rf v n start_interval end_interval)
-//     = LP.append_assoc rf1 rf2 (dimplies_clauses v1 v2 v);
-//       append_valid_cnf_formulas rf1 rf2;
-//       append_valid_cnf_formulas (rf1 @ rf2) (dimplies_clauses v1 v2 v);
-//       // assert (variables_in_interval rf n start_interval end_interval);
-//       // assert (valid (DImplies f1 f2) rf v n start_interval end_interval);
+let and_clauses_in_interval (v1:int) (v2:int) (v:int) (n:nat) (start_interval:nat) (mid:nat) (end_interval:nat)
+    : Lemma (requires n <= start_interval && start_interval <= mid && mid <= v &&
+                      valid_variable v1 && valid_variable v2 && valid_variable v &&
+                      variable_in_interval v1 n start_interval mid &&
+                      variable_in_interval v2 n mid v &&
+                      end_interval = v + 1)
+            (ensures variables_in_interval (and_clauses v1 v2 v) n start_interval end_interval)
+    = ()
 
-//       let aux (tau : list bool) 
-//           : Lemma (requires L.length tau >= end_interval /\
-//                             truth_value_cnf_formula rf tau)
-//                   (ensures truth_value_literal (pos_var_to_lit v) tau = truth_value (DImplies f1 f2) tau)
-//           = assert (variables_up_to_cnf_formula rf (L.length tau));
-//             variables_up_to_monotone f1 n (L.length tau);
-//             variables_up_to_monotone f2 n (L.length tau);
-//             assert (truth_value_literal (pos_var_to_lit v1) tau = truth_value f1 tau);
-//             assert (truth_value_literal (pos_var_to_lit v2) tau = truth_value f2 tau);
-//             lemma_and_clauses v1 v2 v tau;
-//             assert (truth_value_literal (pos_var_to_lit v) tau = truth_value (DImplies f1 f2) tau)
-//       in
-//       forall_intro (move_requires aux)
+
+let prove_same_value_and (f1:formula_t) (rf1 : list (list int)) (v1:int)
+                         (f2:formula_t) (rf2 : list (list int)) (v2:int)
+                         (n:nat) (start_interval:nat) (mid:nat) (end_interval:nat)
+                         (v:int) (rf : list (list int))
+    : Lemma (requires n <= start_interval /\ start_interval <= mid /\ mid <= v /\
+                      valid f1 rf1 v1 n start_interval mid /\
+                      tseitin_same_value f1 rf1 v1 n start_interval mid /\
+                      valid f2 rf2 v2 n mid v /\
+                      tseitin_same_value f2 rf2 v2 n mid v /\
+                      rf = rf1 @ rf2 @ (and_clauses v1 v2 v) /\
+                      end_interval = v + 1)
+            (ensures valid (And f1 f2) rf v n start_interval end_interval /\
+                     tseitin_same_value (And f1 f2) rf v n start_interval end_interval)
+    = LP.append_assoc rf1 rf2 (and_clauses v1 v2 v);
+      append_valid_cnf_formulas rf1 rf2;
+      append_valid_cnf_formulas (rf1 @ rf2) (and_clauses v1 v2 v);
+
+      variables_in_interval_monotone rf1 n start_interval start_interval mid end_interval;
+      variables_in_interval_monotone rf2 n mid start_interval v end_interval;
+
+      and_clauses_in_interval v1 v2 v n start_interval mid end_interval;
+      append_variables_in_interval rf1 rf2 n start_interval end_interval;
+      append_variables_in_interval (rf1 @ rf2) (and_clauses v1 v2 v) n start_interval end_interval;
+
+      assert (valid (And f1 f2) rf v n start_interval end_interval);
+
+      let aux (tau : list bool) 
+          : Lemma (requires L.length tau >= end_interval /\
+                            truth_value_cnf_formula rf tau)
+                  (ensures variables_up_to (And f1 f2) (L.length tau) &&
+                           variables_up_to_literal (pos_var_to_lit v) (L.length tau) &&truth_value_literal (pos_var_to_lit v) tau = truth_value (And f1 f2) tau)
+          = assert (variables_up_to_cnf_formula rf (L.length tau));
+            variables_up_to_monotone f1 n (L.length tau);
+            variables_up_to_monotone f2 n (L.length tau);
+            assert (truth_value_literal (pos_var_to_lit v1) tau = truth_value f1 tau);
+            assert (truth_value_literal (pos_var_to_lit v2) tau = truth_value f2 tau);
+            lemma_and_clauses v1 v2 v tau;
+            assert (truth_value_literal (pos_var_to_lit v) tau = truth_value (And f1 f2) tau)
+      in
+      forall_intro (move_requires aux)
+
+
+let implies_clauses_in_interval (v1:int) (v2:int) (v:int) (n:nat) (start_interval:nat) (mid:nat) (end_interval:nat)
+    : Lemma (requires n <= start_interval && start_interval <= mid && mid <= v &&
+                      valid_variable v1 && valid_variable v2 && valid_variable v &&
+                      variable_in_interval v1 n start_interval mid &&
+                      variable_in_interval v2 n mid v &&
+                      end_interval = v + 1)
+            (ensures variables_in_interval (implies_clauses v1 v2 v) n start_interval end_interval)
+    = ()
+
+
+let prove_same_value_implies (f1:formula_t) (rf1 : list (list int)) (v1:int)
+                             (f2:formula_t) (rf2 : list (list int)) (v2:int)
+                             (n:nat) (start_interval:nat) (mid:nat) (end_interval:nat)
+                             (v:int) (rf : list (list int))
+    : Lemma (requires n <= start_interval /\ start_interval <= mid /\ mid <= v /\
+                      valid f1 rf1 v1 n start_interval mid /\
+                      tseitin_same_value f1 rf1 v1 n start_interval mid /\
+                      valid f2 rf2 v2 n mid v /\
+                      tseitin_same_value f2 rf2 v2 n mid v /\
+                      rf = rf1 @ rf2 @ (implies_clauses v1 v2 v) /\
+                      end_interval = v + 1)
+            (ensures valid (Implies f1 f2) rf v n start_interval end_interval /\
+                     tseitin_same_value (Implies f1 f2) rf v n start_interval end_interval)
+    = LP.append_assoc rf1 rf2 (implies_clauses v1 v2 v);
+      append_valid_cnf_formulas rf1 rf2;
+      append_valid_cnf_formulas (rf1 @ rf2) (implies_clauses v1 v2 v);
+
+      variables_in_interval_monotone rf1 n start_interval start_interval mid end_interval;
+      variables_in_interval_monotone rf2 n mid start_interval v end_interval;
+
+      implies_clauses_in_interval v1 v2 v n start_interval mid end_interval;
+      append_variables_in_interval rf1 rf2 n start_interval end_interval;
+      append_variables_in_interval (rf1 @ rf2) (implies_clauses v1 v2 v) n start_interval end_interval;
+
+      assert (valid (Implies f1 f2) rf v n start_interval end_interval);
+
+      let aux (tau : list bool) 
+          : Lemma (requires L.length tau >= end_interval /\
+                            truth_value_cnf_formula rf tau)
+                  (ensures variables_up_to (Implies f1 f2) (L.length tau) &&
+                           variables_up_to_literal (pos_var_to_lit v) (L.length tau) &&truth_value_literal (pos_var_to_lit v) tau = truth_value (Implies f1 f2) tau)
+          = assert (variables_up_to_cnf_formula rf (L.length tau));
+            variables_up_to_monotone f1 n (L.length tau);
+            variables_up_to_monotone f2 n (L.length tau);
+            assert (truth_value_literal (pos_var_to_lit v1) tau = truth_value f1 tau);
+            assert (truth_value_literal (pos_var_to_lit v2) tau = truth_value f2 tau);
+            lemma_and_clauses v1 v2 v tau;
+            assert (truth_value_literal (pos_var_to_lit v) tau = truth_value (Implies f1 f2) tau)
+      in
+      forall_intro (move_requires aux)
+
+
+let dimplies_clauses_in_interval (v1:int) (v2:int) (v:int) (n:nat) (start_interval:nat) (mid:nat) (end_interval:nat)
+    : Lemma (requires n <= start_interval && start_interval <= mid && mid <= v &&
+                      valid_variable v1 && valid_variable v2 && valid_variable v &&
+                      variable_in_interval v1 n start_interval mid &&
+                      variable_in_interval v2 n mid v &&
+                      end_interval = v + 1)
+            (ensures variables_in_interval (dimplies_clauses v1 v2 v) n start_interval end_interval)
+    = ()
+
+
+let prove_same_value_dimplies (f1:formula_t) (rf1 : list (list int)) (v1:int)
+                              (f2:formula_t) (rf2 : list (list int)) (v2:int)
+                              (n:nat) (start_interval:nat) (mid:nat) (end_interval:nat)
+                              (v:int) (rf : list (list int))
+    : Lemma (requires n <= start_interval /\ start_interval <= mid /\ mid <= v /\
+                      valid f1 rf1 v1 n start_interval mid /\
+                      tseitin_same_value f1 rf1 v1 n start_interval mid /\
+                      valid f2 rf2 v2 n mid v /\
+                      tseitin_same_value f2 rf2 v2 n mid v /\
+                      rf = rf1 @ rf2 @ (dimplies_clauses v1 v2 v) /\
+                      end_interval = v + 1)
+            (ensures valid (DImplies f1 f2) rf v n start_interval end_interval /\
+                     tseitin_same_value (DImplies f1 f2) rf v n start_interval end_interval)
+    = LP.append_assoc rf1 rf2 (dimplies_clauses v1 v2 v);
+      append_valid_cnf_formulas rf1 rf2;
+      append_valid_cnf_formulas (rf1 @ rf2) (dimplies_clauses v1 v2 v);
+
+      variables_in_interval_monotone rf1 n start_interval start_interval mid end_interval;
+      variables_in_interval_monotone rf2 n mid start_interval v end_interval;
+
+      dimplies_clauses_in_interval v1 v2 v n start_interval mid end_interval;
+      append_variables_in_interval rf1 rf2 n start_interval end_interval;
+      append_variables_in_interval (rf1 @ rf2) (dimplies_clauses v1 v2 v) n start_interval end_interval;
+
+      assert (valid (DImplies f1 f2) rf v n start_interval end_interval);
+
+      let aux (tau : list bool) 
+          : Lemma (requires L.length tau >= end_interval /\
+                            truth_value_cnf_formula rf tau)
+                  (ensures variables_up_to (DImplies f1 f2) (L.length tau) &&
+                           variables_up_to_literal (pos_var_to_lit v) (L.length tau) &&truth_value_literal (pos_var_to_lit v) tau = truth_value (DImplies f1 f2) tau)
+          = assert (variables_up_to_cnf_formula rf (L.length tau));
+            variables_up_to_monotone f1 n (L.length tau);
+            variables_up_to_monotone f2 n (L.length tau);
+            assert (truth_value_literal (pos_var_to_lit v1) tau = truth_value f1 tau);
+            assert (truth_value_literal (pos_var_to_lit v2) tau = truth_value f2 tau);
+            lemma_and_clauses v1 v2 v tau;
+            assert (truth_value_literal (pos_var_to_lit v) tau = truth_value (DImplies f1 f2) tau)
+      in
+      forall_intro (move_requires aux)
   
-  
 
-// let prove_can_extend_not (f1:formula_t) (rf1 : list (list int)) (v1:int) (n:nat)
-//                          (start_interval:nat) (v:int) (end_interval:nat) (rf : list (list int))
-//     : Lemma (requires n <= start_interval /\ start_interval <= v /\ v < end_interval /\
-//                       valid f1 rf1 v1 n start_interval v /\
-//                       tseitin_can_extend f1 rf1 v1 n start_interval v /\
-//                       rf = rf1 @ (not_clauses v1 v) /\
-//                       end_interval = v + 1)
-//             (ensures valid (Not f1) rf v n start_interval end_interval /\
-//                      tseitin_can_extend (Not f1) rf v n start_interval end_interval)
-//     = append_valid_cnf_formulas rf1 (not_clauses v1 v);
-//       variables_in_interval_monotone rf1 n start_interval v end_interval;
-//       not_clauses_in_interval v1 v n start_interval end_interval;
-//       append_variables_in_interval rf1 (not_clauses v1 v) n start_interval end_interval;
-//       assert (valid (Not f1) rf v n start_interval end_interval);
+let prove_can_extend_not (f1:formula_t) (rf1 : list (list int)) (v1:int) (n:nat)
+                         (start_interval:nat) (v:int) (end_interval:nat) (rf : list (list int))
+    : Lemma (requires n <= start_interval /\ start_interval <= v /\ v < end_interval /\
+                      valid f1 rf1 v1 n start_interval v /\
+                      tseitin_can_extend f1 rf1 v1 n start_interval v /\
+                      rf = rf1 @ (not_clauses v1 v) /\
+                      end_interval = v + 1)
+            (ensures valid (Not f1) rf v n start_interval end_interval /\
+                     tseitin_can_extend (Not f1) rf v n start_interval end_interval)
+    = append_valid_cnf_formulas rf1 (not_clauses v1 v);
+      variables_in_interval_monotone rf1 n start_interval start_interval v end_interval;
+      not_clauses_in_interval v1 v n start_interval end_interval;
+      append_variables_in_interval rf1 (not_clauses v1 v) n start_interval end_interval;
+      assert (valid (Not f1) rf v n start_interval end_interval);
 
-//       let aux (tau : list bool) 
-//           : Lemma (requires L.length tau = n)
-//                   (ensures L.length tau = n /\
-//                            can_extend tau (Not f1) rf v n start_interval end_interval)
-//           = assert (can_extend tau f1 rf1 v1 n start_interval v);
-//             assert (valid_literal (pos_var_to_lit v1));
+      let aux (tau : list bool) 
+          : Lemma (requires L.length tau = n)
+                  (ensures L.length tau = n /\
+                           can_extend tau (Not f1) rf v n start_interval end_interval)
+          = assert (can_extend tau f1 rf1 v1 n start_interval v);
+            assert (valid_literal (pos_var_to_lit v1));
             
-//             let conditions (tau1 : list bool) =
-//                 is_prefix tau tau1 &&
-//                 L.length tau1 = v &&
-//                 truth_value_cnf_formula rf1 tau1 &&
-//                 truth_value f1 tau = truth_value_literal (pos_var_to_lit v1) tau1
-//             in
-//             assume (exists x . conditions x);
-//             let tau1 = extract_value conditions in
+            let conditions (tau1 : list bool) =
+                is_prefix tau tau1 &&
+                L.length tau1 = v &&
+                truth_value_cnf_formula rf1 tau1 &&
+                truth_value f1 tau = truth_value_literal (pos_var_to_lit v1) tau1
+            in
+            assume (exists x . conditions x);
+            let tau1 = extract_value conditions in
 
-//             negate_literal v1 tau1;
+            negate_literal v1 tau1;
 
-//             let tau' = combine1 tau tau1 n start_interval v (truth_value (Not f1) tau) in
-//             is_prefix_then_is_interval tau tau1;
-//             transfer_truth_value rf1 tau1 tau' n start_interval v;
+            let tau' = combine1 tau tau1 n start_interval v (truth_value (Not f1) tau) in
+            is_prefix_then_is_interval tau tau1;
+            transfer_truth_value rf1 tau1 tau' n start_interval v;
 
-//             transfer_truth_value_lit (pos_var_to_lit v1) tau1 tau' n start_interval v;
-//             assert (truth_value_literal (pos_var_to_lit v1) tau' = truth_value f1 tau);
-//             transfer_truth_value_lit (neg_var_to_lit v1) tau1 tau' n start_interval v;
-//             assert (truth_value_literal (neg_var_to_lit v1) tau1 = not (truth_value_literal (pos_var_to_lit v1) tau1));
+            transfer_truth_value_lit (pos_var_to_lit v1) tau1 tau' n start_interval v;
+            assert (truth_value_literal (pos_var_to_lit v1) tau' = truth_value f1 tau);
+            transfer_truth_value_lit (neg_var_to_lit v1) tau1 tau' n start_interval v;
+            assert (truth_value_literal (neg_var_to_lit v1) tau1 = not (truth_value_literal (pos_var_to_lit v1) tau1));
 
-//             lemma_not_clauses v1 v tau'
-//       in
-//       forall_intro (move_requires aux) 
+            lemma_not_clauses v1 v tau'
+      in
+      forall_intro (move_requires aux) 
 
 
-// let prove_can_extend_or (f1:formula_t) (rf1 : list (list int)) (v1:int) 
-//                         (f2:formula_t) (rf2 : list (list int)) (v2:int) 
-//                         (n:nat) (start_interval:nat) (mid:nat) (v:int) (end_interval:nat)
-//                         (rf :list (list int))
-//     : Lemma (requires n <= start_interval /\ start_interval <= mid /\ mid <= v /\
-//                       valid f1 rf1 v1 n start_interval mid /\
-//                       tseitin_can_extend f1 rf1 v1 n start_interval mid /\
-//                       valid f2 rf2 v2 n mid v /\
-//                       tseitin_can_extend f2 rf2 v2 n mid v /\
-//                       rf = rf1 @ rf2 @ (or_clauses v1 v2 v) /\
-//                       end_interval = v + 1)
-//             (ensures valid (Or f1 f2) rf v n start_interval end_interval /\
-//                      tseitin_can_extend (Or f1 f2) rf v n start_interval end_interval)
-//     = assert (valid (Or f1 f2) rf v n start_interval end_interval);
-//       let aux (tau : list bool)
-//           : Lemma (requires L.length tau = n)
-//                   (ensures can_extend tau (Or f1 f2) rf v n start_interval end_interval)
-//           = let conditions (tau1 : list bool) =
-//                 // tau <= tau1 /\
-//                 L.length tau1 = mid /\
-//                 truth_value_cnf_formula rf1 tau1 /\
-//                 truth_value f1 tau = truth_value_literal (pos_var_to_lit v1) tau1
-//             in
-//             let extract_from_exists : (tau1 : list bool {conditions tau1}) -> prop = fun (tau1 : list bool) -> conditions tau1 in
-//             let tau1 : list bool = FStar.IndefiniteDescription.indefinite_description_ghost (list bool) extract_from_exists in
+#set-options "--split_queries always"
+let prove_can_extend_or (f1:formula_t) (rf1 : list (list int)) (v1:nat) 
+                        (f2:formula_t) (rf2 : list (list int)) (v2:nat) 
+                        (n:nat) (start_interval:nat) (mid:nat) (v:nat) (end_interval:nat)
+                        (rf :list (list int))
+    : Lemma (requires n <= start_interval /\ start_interval <= mid /\ mid <= v /\
+                      valid f1 rf1 v1 n start_interval mid /\
+                      tseitin_can_extend f1 rf1 v1 n start_interval mid /\
+                      valid f2 rf2 v2 n mid v /\
+                      tseitin_can_extend f2 rf2 v2 n mid v /\
+                      rf = rf1 @ rf2 @ (or_clauses v1 v2 v) /\
+                      end_interval = v + 1)
+            (ensures valid (Or f1 f2) rf v n start_interval end_interval /\
+                     tseitin_can_extend (Or f1 f2) rf v n start_interval end_interval)
+    = LP.append_assoc rf1 rf2 (or_clauses v1 v2 v);
+      append_valid_cnf_formulas rf1 rf2;
+      append_valid_cnf_formulas (rf1 @ rf2) (or_clauses v1 v2 v);
 
-//             let conditions (tau2 : list bool) =
-//                 // tau <= tau2 /\
-//                 L.length tau2 = v /\
-//                 truth_value_cnf_formula rf2 tau2 /\
-//                 truth_value f2 tau = truth_value_literal (pos_var_to_lit v2) tau2
-//             in
-//             let extract_from_exists : (tau2 : list bool {conditions tau2}) -> prop = fun (tau2 : list bool) -> conditions tau2 in
-//             let tau2 : list bool = FStar.IndefiniteDescription.indefinite_description_ghost (list bool) extract_from_exists in
+      variables_in_interval_monotone rf1 n start_interval start_interval mid end_interval;
+      variables_in_interval_monotone rf2 n mid start_interval v end_interval;
 
-//             let tau' = combine tau tau1 tau2 n start_interval mid v (truth_value (Or f1 f2) tau) in
+      or_clauses_in_interval v1 v2 v n start_interval mid end_interval;
+      append_variables_in_interval rf1 rf2 n start_interval end_interval;
+      append_variables_in_interval (rf1 @ rf2) (or_clauses v1 v2 v) n start_interval end_interval;
+      
+      assert (valid (Or f1 f2) rf v n start_interval end_interval);
 
-//             assert (interval_of_list tau' 0 n = interval_of_list tau 0 n);
-//             assert (interval_of_list tau' start_interval mid = interval_of_list tau1 start_interval mid);
-//             assert (interval_of_list tau' mid v = interval_of_list tau2 mid v);
-//             assert (L.index tau' v = truth_value (Or f1 f2) tau);
+      let aux (tau : list bool)
+          : Lemma (requires L.length tau = n)
+                  (ensures L.length tau = n /\
+                           can_extend tau (Or f1 f2) rf v n start_interval end_interval)
+          = let conditions1 (tau1 : list bool) =
+                is_prefix tau tau1 &&
+                L.length tau1 = mid &&
+                truth_value_cnf_formula rf1 tau1 &&
+                truth_value f1 tau = truth_value_literal (pos_var_to_lit v1) tau1
+            in
+            assume (exists x . conditions1 x);
+            let tau1 = extract_value conditions1 in
+            assert (is_prefix tau tau1);
+            assert (L.length tau1 = mid);
 
-//             assert (truth_value_literal (pos_var_to_lit v) tau' = truth_value (Or f1 f2) tau);
-//             assert (truth_value_literal (neg_var_to_lit v) tau' = not (truth_value (Or f1 f2) tau));
+            let conditions2 (tau2 : list bool) =
+                is_prefix tau tau2 &&
+                L.length tau2 = v &&
+                truth_value_cnf_formula rf2 tau2 &&
+                truth_value f2 tau = truth_value_literal (pos_var_to_lit v2) tau2
+            in
+            assume (exists x . conditions2 x);
+            let tau2 = extract_value conditions2 in
+            assert (is_prefix tau tau2);
+            assert (L.length tau2 = v);
 
-//             transfer_truth_value rf1 tau1 tau' n start_interval mid;
-//             transfer_truth_value rf2 tau2 tau' n mid v;
+            let tau' = combine tau tau1 tau2 n start_interval mid v (truth_value (Or f1 f2) tau) in
+            assert (L.length tau' = v + 1);
 
-//             transfer_truth_value_lit (pos_var_to_lit v1) tau1 tau' n start_interval mid;
-//             transfer_truth_value_lit (neg_var_to_lit v1) tau1 tau' n start_interval mid;
-//             assert (truth_value_literal (pos_var_to_lit v1) tau' = truth_value f1 tau);
-//             assert (truth_value_literal (neg_var_to_lit v1) tau' = not (truth_value f1 tau));
+            // assert (interval_of_list tau' 0 n = interval_of_list tau 0 n);
+            assert (interval_of_list tau' start_interval mid = interval_of_list tau1 start_interval mid);
+            assert (interval_of_list tau' mid v = interval_of_list tau2 mid v);
+            assert (L.index tau' v = truth_value (Or f1 f2) tau);
 
-//             transfer_truth_value_lit (pos_var_to_lit v2) tau2 tau' n mid v;
-//             transfer_truth_value_lit (neg_var_to_lit v2) tau2 tau' n mid v;
-//             assert (truth_value_literal (pos_var_to_lit v2) tau' = truth_value f2 tau);
-//             assert (truth_value_literal (neg_var_to_lit v2) tau' = not (truth_value f2 tau));
+            assert (truth_value_literal (pos_var_to_lit v) tau' = truth_value (Or f1 f2) tau);
+            assert (truth_value_literal (neg_var_to_lit v) tau' = not (truth_value (Or f1 f2) tau));
 
-//             assert (truth_value (Or f1 f2) tau = truth_value f1 tau || truth_value f2 tau);
-//             lemma_or_clauses v1 v2 v tau';
-//             assert (can_extend tau (Or f1 f2) rf v n start_interval end_interval)
-//       in
-//       forall_intro (move_requires aux)
+            is_prefix_then_is_interval tau tau1;
+            transfer_truth_value rf1 tau1 tau' n start_interval mid;
+            is_prefix_then_is_interval tau tau2;
+            transfer_truth_value rf2 tau2 tau' n mid v;
+
+            transfer_truth_value_lit (pos_var_to_lit v1) tau1 tau' n start_interval mid;
+            // assert (truth_value_literal (pos_var_to_lit v1) tau' = truth_value f1 tau);
+            transfer_truth_value_lit (neg_var_to_lit v1) tau1 tau' n start_interval mid;
+            // assert (truth_value_literal (neg_var_to_lit v1) tau' = not (truth_value f1 tau));
+
+            transfer_truth_value_lit (pos_var_to_lit v2) tau2 tau' n mid v;
+            // assert (truth_value_literal (pos_var_to_lit v2) tau' = truth_value f2 tau);
+            transfer_truth_value_lit (neg_var_to_lit v2) tau2 tau' n mid v;
+            // assert (truth_value_literal (neg_var_to_lit v2) tau' = not (truth_value f2 tau));
+
+            // assert (truth_value (Or f1 f2) tau = truth_value f1 tau || truth_value f2 tau);
+            lemma_or_clauses v1 v2 v tau';
+            assert (can_extend tau (Or f1 f2) rf v n start_interval end_interval)
+      in
+      forall_intro (move_requires aux)
+
+
+let prove_can_extend_and (f1:formula_t) (rf1 : list (list int)) (v1:nat) 
+                         (f2:formula_t) (rf2 : list (list int)) (v2:nat) 
+                         (n:nat) (start_interval:nat) (mid:nat) (v:nat) (end_interval:nat)
+                         (rf :list (list int))
+    : Lemma (requires n <= start_interval /\ start_interval <= mid /\ mid <= v /\
+                      valid f1 rf1 v1 n start_interval mid /\
+                      tseitin_can_extend f1 rf1 v1 n start_interval mid /\
+                      valid f2 rf2 v2 n mid v /\
+                      tseitin_can_extend f2 rf2 v2 n mid v /\
+                      rf = rf1 @ rf2 @ (and_clauses v1 v2 v) /\
+                      end_interval = v + 1)
+            (ensures valid (And f1 f2) rf v n start_interval end_interval /\
+                     tseitin_can_extend (And f1 f2) rf v n start_interval end_interval)
+    = LP.append_assoc rf1 rf2 (and_clauses v1 v2 v);
+      append_valid_cnf_formulas rf1 rf2;
+      append_valid_cnf_formulas (rf1 @ rf2) (and_clauses v1 v2 v);
+
+      variables_in_interval_monotone rf1 n start_interval start_interval mid end_interval;
+      variables_in_interval_monotone rf2 n mid start_interval v end_interval;
+
+      and_clauses_in_interval v1 v2 v n start_interval mid end_interval;
+      append_variables_in_interval rf1 rf2 n start_interval end_interval;
+      append_variables_in_interval (rf1 @ rf2) (and_clauses v1 v2 v) n start_interval end_interval;
+      assert (valid (And f1 f2) rf v n start_interval end_interval);
+      
+      let aux (tau : list bool)
+          : Lemma (requires L.length tau = n)
+                  (ensures L.length tau = n /\
+                           can_extend tau (And f1 f2) rf v n start_interval end_interval)
+          = let conditions1 (tau1 : list bool) : Tot bool =
+                is_prefix tau tau1 &&
+                L.length tau1 = mid &&
+                truth_value_cnf_formula rf1 tau1 &&
+                truth_value f1 tau = truth_value_literal (pos_var_to_lit v1) tau1
+            in
+            assume (exists x . conditions1 x);
+            let tau1 = extract_value conditions1 in
+            assert (is_prefix tau tau1);
+            assert (L.length tau1 = mid);
+
+
+            let conditions2 (tau2 : list bool) : Tot bool =
+                is_prefix tau tau2 &&
+                L.length tau2 = v &&
+                truth_value_cnf_formula rf2 tau2 &&
+                truth_value f2 tau = truth_value_literal (pos_var_to_lit v2) tau2
+            in
+            assume (exists x . conditions2 x);
+            let tau2 = extract_value conditions2 in
+            assert (is_prefix tau tau2);
+            assert (L.length tau2 = v);
+
+
+            let tau' = combine tau tau1 tau2 n start_interval mid v (truth_value (And f1 f2) tau) in
+            assert (L.length tau' = v + 1);
+
+            // assert (interval_of_list tau' 0 n = interval_of_list tau 0 n);
+            assert (interval_of_list tau' start_interval mid = interval_of_list tau1 start_interval mid);
+            assert (interval_of_list tau' mid v = interval_of_list tau2 mid v);
+            assert (L.index tau' v = truth_value (And f1 f2) tau);
+
+            assert (truth_value_literal (pos_var_to_lit v) tau' = truth_value (And f1 f2) tau);
+            assert (truth_value_literal (neg_var_to_lit v) tau' = not (truth_value (And f1 f2) tau));
+
+            is_prefix_then_is_interval tau tau1;
+            transfer_truth_value rf1 tau1 tau' n start_interval mid;
+            is_prefix_then_is_interval tau tau2;
+            transfer_truth_value rf2 tau2 tau' n mid v;
+
+            transfer_truth_value_lit (pos_var_to_lit v1) tau1 tau' n start_interval mid;
+            // assert (truth_value_literal (pos_var_to_lit v1) tau' = truth_value f1 tau);
+            transfer_truth_value_lit (neg_var_to_lit v1) tau1 tau' n start_interval mid;
+            // assert (truth_value_literal (neg_var_to_lit v1) tau' = not (truth_value f1 tau));
+            
+            transfer_truth_value_lit (pos_var_to_lit v2) tau2 tau' n mid v;
+            // assert (truth_value_literal (pos_var_to_lit v2) tau' = truth_value f2 tau);
+            transfer_truth_value_lit (neg_var_to_lit v2) tau2 tau' n mid v;
+            // assert (truth_value_literal (neg_var_to_lit v2) tau' = not (truth_value f1 tau));
+
+            lemma_and_clauses v1 v2 v tau';
+            assert (can_extend tau (And f1 f2) rf v n start_interval end_interval)
+      in
+      forall_intro (move_requires aux)
+
+
+let prove_can_extend_implies (f1:formula_t) (rf1 : list (list int)) (v1:nat) 
+                             (f2:formula_t) (rf2 : list (list int)) (v2:nat) 
+                             (n:nat) (start_interval:nat) (mid:nat) (v:nat) (end_interval:nat)
+                             (rf :list (list int))
+    : Lemma (requires n <= start_interval /\ start_interval <= mid /\ mid <= v /\
+                      valid f1 rf1 v1 n start_interval mid /\
+                      tseitin_can_extend f1 rf1 v1 n start_interval mid /\
+                      valid f2 rf2 v2 n mid v /\
+                      tseitin_can_extend f2 rf2 v2 n mid v /\
+                      rf = rf1 @ rf2 @ (implies_clauses v1 v2 v) /\
+                      end_interval = v + 1)
+            (ensures valid (Implies f1 f2) rf v n start_interval end_interval /\
+                     tseitin_can_extend (Implies f1 f2) rf v n start_interval end_interval)
+    = LP.append_assoc rf1 rf2 (implies_clauses v1 v2 v);
+      append_valid_cnf_formulas rf1 rf2;
+      append_valid_cnf_formulas (rf1 @ rf2) (implies_clauses v1 v2 v);
+
+      variables_in_interval_monotone rf1 n start_interval start_interval mid end_interval;
+      variables_in_interval_monotone rf2 n mid start_interval v end_interval;
+
+      implies_clauses_in_interval v1 v2 v n start_interval mid end_interval;
+      append_variables_in_interval rf1 rf2 n start_interval end_interval;
+      append_variables_in_interval (rf1 @ rf2) (implies_clauses v1 v2 v) n start_interval end_interval;
+      
+      assert (valid (Implies f1 f2) rf v n start_interval end_interval);
+
+      let aux (tau : list bool) 
+          : Lemma (requires L.length tau = n)
+                  (ensures L.length tau = n /\
+                           can_extend tau (Implies f1 f2) rf v n start_interval end_interval)
+          = let conditions1 (tau1 : list bool) : Tot bool =
+                is_prefix tau tau1 &&
+                L.length tau1 = mid &&
+                truth_value_cnf_formula rf1 tau1 &&
+                truth_value f1 tau = truth_value_literal (pos_var_to_lit v1) tau1
+            in
+            assume (exists x . conditions1 x);
+            let tau1 = extract_value conditions1 in
+            assert (is_prefix tau tau1);
+            assert (L.length tau1 = mid);
+
+            let conditions2 (tau2 : list bool) : Tot bool =
+                is_prefix tau tau2 &&
+                L.length tau2 = v &&
+                truth_value_cnf_formula rf2 tau2 &&
+                truth_value f2 tau = truth_value_literal (pos_var_to_lit v2) tau2
+            in
+            assume (exists x . conditions2 x);
+            let tau2 = extract_value conditions2 in
+            assert (is_prefix tau tau2);
+            assert (L.length tau2 = v);
+
+
+            let tau' = combine tau tau1 tau2 n start_interval mid v (truth_value (Implies f1 f2) tau) in
+            assert (L.length tau' = v + 1);
+
+            // assert (interval_of_list tau' 0 n = interval_of_list tau 0 n);
+            assert (interval_of_list tau' start_interval mid = interval_of_list tau1 start_interval mid);
+            assert (interval_of_list tau' mid v = interval_of_list tau2 mid v);
+            assert (L.index tau' v = truth_value (Implies f1 f2) tau);
+
+            assert (truth_value_literal (pos_var_to_lit v) tau' = truth_value (Implies f1 f2) tau);
+            assert (truth_value_literal (neg_var_to_lit v) tau' = not (truth_value (Implies f1 f2) tau));
+
+            is_prefix_then_is_interval tau tau1;
+            transfer_truth_value rf1 tau1 tau' n start_interval mid;
+            is_prefix_then_is_interval tau tau2;
+            transfer_truth_value rf2 tau2 tau' n mid v;
+
+            transfer_truth_value_lit (pos_var_to_lit v1) tau1 tau' n start_interval mid;
+            // assert (truth_value_literal (pos_var_to_lit v1) tau' = truth_value f1 tau);
+            transfer_truth_value_lit (neg_var_to_lit v1) tau1 tau' n start_interval mid;
+            // assert (truth_value_literal (neg_var_to_lit v1) tau' = not (truth_value f1 tau));
+            
+            transfer_truth_value_lit (pos_var_to_lit v2) tau2 tau' n mid v;
+            // assert (truth_value_literal (pos_var_to_lit v2) tau' = truth_value f2 tau);
+            transfer_truth_value_lit (neg_var_to_lit v2) tau2 tau' n mid v;
+            // assert (truth_value_literal (neg_var_to_lit v2) tau' = not (truth_value f1 tau));
+
+            // assert (truth_value (Implies f1 f2) tau = (truth_value f1 tau ==> truth_value f2 tau));
+
+            lemma_implies_clauses v1 v2 v tau';
+            assert (can_extend tau (Implies f1 f2) rf v n start_interval end_interval)
+      in
+      forall_intro (move_requires aux)
+#reset-options
